mem_force no longer flattens the entire subobject for "unsigned char" addresses.
The operation "mem_force Γ m a" used to apply the identify function to
pricisely the object "a", even in case "a" is an "unsigned char" address
refering to an individual byte. This caused the ctree substructure of the
entire subobject to disappear and had the undesired effect that:

  mem_force Γ a m ⊑{Γ,true@Γm} m

failed to hold (i.e. unused reads cannot be removed).

memory.v
@@ -13,7 +13,7 @@ Section memory_operations.
     guard (ctree_Forall (λ xb, Some Readable ⊆ pbit_kind xb) w);
     Some (to_val Γ w).
   Definition mem_force (Γ : env Ti) (a : addr Ti) : mem Ti → mem Ti :=
-    cmap_alter Γ id a.
+    cmap_alter_ref Γ id (addr_index a) (addr_ref Γ a).
 
   Definition mem_writable (Γ : env Ti) (a : addr Ti) (m : mem Ti) : Prop :=
     ∃ w, m !!{Γ} a = Some w
@@ -106,9 +106,6 @@ Implicit Types βs : list bool.
 Implicit Types xb : pbit Ti.
 Implicit Types xbs : list (pbit Ti).
 Implicit Types Ω : lockset.
-
-Local Opaque nmap.Nempty.
-Arguments cmap_lookup _ _ _ !_ !_ /.
 
 Hint Resolve Forall_app_2 Forall2_app.
 Hint Immediate cmap_lookup_typed val_typed_type_valid.
@@ -247,7 +244,7 @@ Lemma mem_alloc_writable_top Γ m o malloc τ :
   mem_allocable o m → mem_writable Γ (addr_top o τ) (mem_alloc Γ o malloc τ m).
 Proof.
   unfold mem_allocable. intros. exists (ctree_new Γ pbit_full τ); split.
-  * unfold lookupE, cmap_lookup. 
+  * unfold lookupE, cmap_lookup.
     rewrite option_guard_True by eauto using addr_top_strict.
     by destruct m as [m]; simplify_map_equality'.
   * apply ctree_new_Forall; auto; by destruct alloc.
@@ -415,9 +412,9 @@ Proof. unfold lookupE, mem_lookup. by rewrite cmap_lookup_erase. Qed.
 Lemma mem_force_memenv_of Γ Γm m a :
   ✓ Γ → ✓{Γ,Γm} m → is_Some (m !!{Γ} a) → '{mem_force Γ a m} = '{m}.
 Proof.
-  unfold mem_force, lookupE, mem_lookup. intros ?? [v ?].
-  destruct (m !!{Γ} a) as [w|] eqn:?; simplify_equality'.
-  by erewrite cmap_alter_memenv_of by eauto.
+  unfold mem_force, lookupE, mem_lookup; simpl; unfold lookupE, cmap_lookup.
+  intros ?? [v ?]. by destruct (m !!{Γ} _) as [w|] eqn:?;
+    simplify_option_equality; eauto using cmap_alter_ref_memenv_of.
 Qed.
 Lemma mem_force_forward Γ Γm m a :
   ✓ Γ → ✓{Γ,Γm} m → is_Some (m !!{Γ} a) → '{m} ⇒ₘ '{mem_force Γ a m}.
@@ -425,10 +422,19 @@ Proof. intros. by erewrite mem_force_memenv_of by eauto. Qed.
 Lemma mem_force_valid Γ Γm m a :
   ✓ Γ → ✓{Γ,Γm} m → is_Some (m !!{Γ} a) → ✓{Γ,Γm} (mem_force Γ a m).
 Proof.
-  unfold mem_force, lookupE, mem_lookup. intros ?? [v ?].
-  destruct (m !!{Γ} a) as [w|] eqn:?; simplify_option_equality.
-  eapply cmap_alter_valid; eauto using cmap_lookup_Some,
-    ctree_Forall_not, cmap_lookup_Some, pbits_mapped.
+  unfold mem_force, lookupE, mem_lookup; simpl; unfold lookupE, cmap_lookup.
+  intros ?? [v ?]; case_option_guard; simplify_equality';
+    destruct (m !!{Γ} _) as [w|] eqn:?; simplify_equality'.
+  destruct (cmap_lookup_ref_Some Γ Γm m (addr_index a)
+    (addr_ref Γ a) w) as (?&?&?&?&?); eauto.
+  eapply cmap_alter_ref_valid; eauto.
+  { eapply type_of_typed; eauto. }
+  case_decide; simplify_equality'; case_option_guard; simplify_equality'.
+  { eapply ctree_Forall_not; eauto using pbits_mapped. }
+  destruct (w !!{Γ} _) as [w'|] eqn:?; simplify_option_equality.
+  intros ?; eapply (ctree_Forall_not _ _ _ w');
+    eauto using ctree_lookup_byte_Forall, pbit_unmapped_indetify,
+    pbits_mapped, ctree_lookup_byte_typed.
 Qed.
 Lemma mem_force_valid' Γ m a :
   ✓ Γ → ✓{Γ} m → is_Some (m !!{Γ} a) → ✓{Γ} (mem_force Γ a m).
@@ -438,33 +444,38 @@ Proof.
 Qed.
 Lemma mem_erase_force Γ m a :
   cmap_erase (mem_force Γ a m) = mem_force Γ a (cmap_erase m).
-Proof. apply cmap_erase_alter. Qed.
+Proof. apply cmap_erase_alter_ref. Qed.
 Lemma mem_lookup_force Γ Γm m a v τ :
   ✓ Γ → ✓{Γ,Γm} m → (Γ,Γm) ⊢ a : Some τ → m !!{Γ} a = Some v → addr_is_obj a →
   mem_force Γ a m !!{Γ} a = Some v.
 Proof.
-  unfold lookupE, mem_lookup, mem_force. intros.
-  destruct (m !!{Γ} a) as [w'|] eqn:?; simplify_equality'.
-  by erewrite cmap_lookup_alter by eauto; simplify_option_equality.
+  unfold mem_force, lookupE, mem_lookup; simpl; unfold lookupE, cmap_lookup.
+  intros; case_option_guard; simplify_equality';
+    destruct (m !!{Γ} _) as [w|] eqn:?; simplify_equality'.
+  by erewrite cmap_lookup_ref_alter by
+    eauto using cmap_lookup_ref_le, ref_freeze_le_r; simplify_option_equality.
 Qed.
 Lemma mem_lookup_force_disjoint Γ Γm m a1 a2 τ2 v1 :
-  ✓ Γ → ✓{Γ,Γm} m → a1 ⊥{Γ} a2 → m !!{Γ} a1 = Some v1 → (Γ,Γm) ⊢ a2 : Some τ2 →
-  is_Some (m !!{Γ} a2) → mem_force Γ a2 m !!{Γ} a1 = Some v1.
+  ✓ Γ → ✓{Γ,Γm} m → a1 ⊥{Γ} a2 → m !!{Γ} a1 = Some v1 →
+  mem_force Γ a2 m !!{Γ} a1 = Some v1.
 Proof.
-  unfold lookupE, mem_force, mem_lookup. intros ????? [??].
-  destruct (m !!{Γ} a1) as [w1|] eqn:?,
-    (m !!{Γ} a2) as [w2|] eqn:?; simplify_equality'.
-  by erewrite cmap_lookup_alter_disjoint by eauto.
+  unfold mem_force, lookupE, mem_lookup; simpl; unfold lookupE, cmap_lookup.
+  intros ?? Ha ?; case_option_guard; simplify_equality'.
+  destruct (m !!{Γ} (addr_index a1,_)) as [w1|] eqn:?; simplify_equality'.
+  destruct Ha as [|[[??]|(<-&?&?&?&?)]];
+    erewrite ?cmap_lookup_ref_alter_disjoint by eauto; auto.
+  by erewrite cmap_lookup_ref_alter
+    by eauto using cmap_lookup_ref_le, ref_freeze_le_r.
 Qed.
-Lemma mem_force_commute Γ Γm m a1 a2 τ1 τ2 :
-  ✓ Γ → ✓{Γ,Γm} m → a1 ⊥{Γ} a2 →
-  (Γ,Γm) ⊢ a1 : Some τ1 → is_Some (m !!{Γ} a1) →
-  (Γ,Γm) ⊢ a2 : Some τ2 → is_Some (m !!{Γ} a2) →
+Lemma mem_force_commute Γ m a1 a2 :
+  a1 ⊥{Γ} a2 →
   mem_force Γ a1 (mem_force Γ a2 m) = mem_force Γ a2 (mem_force Γ a1 m).
 Proof.
-  unfold lookupE, mem_lookup, mem_force. intros ???? [??] ? [??].
-  destruct (m !!{Γ} a1) as [w1|] eqn:?, (m !!{Γ} a2) as [w2|] eqn:?;
-    simplify_equality'; eauto using cmap_alter_commute.
+  unfold mem_force; intros [?|[[??]|(<-&Hr&?&?&?)]];
+    auto using cmap_alter_ref_commute.
+  by rewrite <-!(cmap_alter_ref_le _ _ _ _ (addr_ref Γ a1)), !Hr,
+    !(cmap_alter_ref_le _ _ _ (freeze true <$> addr_ref Γ a2) (addr_ref Γ a2)),
+    <-!cmap_alter_ref_compose by eauto using ref_freeze_le_l.
 Qed.
 
 (** Properties of the [insert] function *)
@@ -475,7 +486,8 @@ Lemma mem_writable_alive Γ Γm m a :
 Proof.
   intros ? Hm (w&?&?).
   assert ((Γ,Γm) ⊢ w : type_of w) by eauto using cmap_lookup_Some.
-  unfold lookupE, cmap_lookup in *; case_option_guard; simplify_equality'.
+  unfold lookupE, cmap_lookup, lookupE, cmap_lookup_ref in *;
+    case_option_guard; simplify_equality'.
   destruct (cmap_car m !! addr_index a) as [[|w' β]|] eqn:?; simplify_equality'.
   destruct (cmap_valid_Obj Γ Γm m (addr_index a) w' β) as (τ&?&?&?); auto.
 Qed.
@@ -586,15 +598,20 @@ Lemma mem_insert_commute Γ Γm m a1 a2 v1 v2 τ1 τ2 :
   (Γ,Γm) ⊢ a2 : Some τ2 → mem_writable Γ a2 m → (Γ,Γm) ⊢ v2 : τ2 →
   <[a1:=v1]{Γ}>(<[a2:=v2]{Γ}>m) = <[a2:=v2]{Γ}>(<[a1:=v1]{Γ}>m).
 Proof. intros ???? (?&?&?) ?? (?&?&?) ?. eapply cmap_alter_commute; eauto. Qed.
-Lemma mem_insert_force_commute Γ Γm m a1 a2 v1 τ1 τ2 :
-  ✓ Γ → ✓{Γ,Γm} m → a1 ⊥{Γ} a2 →
-  (Γ,Γm) ⊢ a1 : Some τ1 → mem_writable Γ a1 m → (Γ,Γm) ⊢ v1 : τ1 →
-  (Γ,Γm) ⊢ a2 : Some τ2 → is_Some (m !!{Γ} a2) →
+Lemma mem_insert_force_commute Γ m a1 a2 v1 :
+  a1 ⊥{Γ} a2 →
   <[a1:=v1]{Γ}>(mem_force Γ a2 m) = mem_force Γ a2 (<[a1:=v1]{Γ}>m).
 Proof.
-  unfold lookupE, mem_lookup, mem_force. intros ???? (?&?&?) ?? [??].
-  destruct (m !!{Γ} a2) as [w2|] eqn:?; simplify_equality'.
-  eapply cmap_alter_commute; eauto.
+  unfold mem_force, insertE, mem_insert, cmap_alter.
+  intros [?|[[??]|(<-&Hr&?&?&?)]]; auto using cmap_alter_ref_commute.
+  by rewrite <-!(cmap_alter_ref_le _ _ _ _ (addr_ref Γ a1)), !Hr,
+    !(cmap_alter_ref_le _ _ _ (freeze true <$> addr_ref Γ a2) (addr_ref Γ a2)),
+    <-!cmap_alter_ref_compose by eauto using ref_freeze_le_l.
+Qed.
+Lemma mem_insert_force Γ m a v : <[a:=v]{Γ}>(mem_force Γ a m) = <[a:=v]{Γ}>m.
+Proof.
+  unfold insertE, mem_insert, mem_force, cmap_alter.
+  by rewrite <-cmap_alter_ref_compose.
 Qed.
 Lemma mem_insert_writable Γ Γm m a1 a2 v2 τ2 :
   ✓ Γ → ✓{Γ,Γm} m → a1 = a2 ∨ a1 ⊥{Γ} a2 →
@@ -741,10 +758,10 @@ Proof.
   by apply Forall_true.
 Qed.
 Lemma mem_force_singleton Γ Γm a malloc x v τ :
-  ✓ Γ → (Γ,Γm) ⊢ a : Some τ → addr_is_obj a → addr_strict Γ a →
+  ✓ Γ → (Γ,Γm) ⊢ a : Some τ → addr_strict Γ a →
   mem_force Γ a (mem_singleton Γ a malloc x v)
   = mem_singleton Γ a malloc x v.
-Proof. by apply (cmap_alter_singleton _ Γm id _ _ _ τ). Qed.
+Proof. apply (cmap_alter_ref_singleton _ Γm id _ _ _ τ). Qed.
 Lemma mem_insert_singleton Γ Γm a malloc x v1 v2 τ :
   ✓ Γ → (Γ,Γm) ⊢ a : Some τ → addr_is_obj a → addr_strict Γ a →
   (Γ,Γm) ⊢ v1 : τ → (Γ,Γm) ⊢ v2 : τ →
@@ -976,6 +993,40 @@ Proof.
   destruct (decide (o = o')); simplify_map_equality'; split; try done.
   rewrite fmap_Some; intros ([x b]&?&?); decompose_Forall_hyps.
 Qed.
+Lemma mem_locks_alter_ref Γ Γm g o r m w τ σ o' i :
+  ✓Γ → ✓{Γ,Γm} m → Γm ⊢ o : τ → Γ ⊢ r : τ ↣ σ →
+  m !!{Γ} (o,r) = Some w → (Γ,Γm) ⊢ g w : σ →
+  (o',i) ∈ mem_locks (cmap_alter_ref Γ g o r m) ↔
+    (o',i) ∈ mem_locks m ∧ o' ≠ o ∨
+    (o',i) ∈ mem_locks m ∧ o' = o ∧ i < ref_object_offset Γ r ∨
+    o' = o ∧
+      ref_object_offset Γ r ≤ i < ref_object_offset Γ r + bit_size_of Γ σ ∧
+      pbit_locked <$> ctree_flatten (g w)
+      !! (i - ref_object_offset Γ r) = Some true ∨
+    (o',i) ∈ mem_locks m ∧ o' = o ∧
+      ref_object_offset Γ r + bit_size_of Γ σ ≤ i.
+Proof.
+  unfold lookupE, cmap_lookup_ref; intros ? Hm ????; simplify_equality'.
+  destruct (cmap_car m !! o) as [[|w' β]|] eqn:?; simplify_equality'.
+  destruct (cmap_valid_Obj Γ Γm m o w' β) as (τ'&?&_&?&_); auto.
+  rewrite !elem_of_mem_locks; destruct m as [m]; simplify_equality'.
+  destruct (decide (o = o')); simplify_map_equality';
+    [rewrite or_r by tauto|destruct (m !! o) as [[]|]; naive_solver].
+  simplify_type_equality. unfold pbit_locked.
+  erewrite <-!list_lookup_fmap, !list_fmap_compose, ctree_alter_perm_flatten,
+    !list_lookup_fmap by eauto using ctree_lookup_typed.
+  assert (ref_object_offset Γ r + bit_size_of Γ σ ≤ bit_size_of Γ τ)
+    by eauto using ref_object_offset_size'.
+  destruct (le_lt_dec (ref_object_offset Γ r) i);
+    [|rewrite lookup_app_l, lookup_take by solve_length; intuition lia].
+  rewrite lookup_app_r, take_length_le by solve_length.
+  destruct (le_lt_dec (ref_object_offset Γ r + bit_size_of Γ σ) i);
+    [|rewrite lookup_app_l by auto; intuition omega].
+  erewrite lookup_app_r, ctree_flatten_length, lookup_drop by eauto.
+  replace (ref_object_offset Γ r + bit_size_of Γ σ
+    + (i - ref_object_offset Γ r - bit_size_of Γ σ)) with i by lia.
+  intuition lia.
+Qed.
 Lemma mem_locks_alter Γ Γm g a m w τ o i :
   ✓Γ → ✓{Γ,Γm} m → (Γ,Γm) ⊢ a : Some τ → m !!{Γ} a = Some w → (Γ,Γm) ⊢ g w : τ →
   (o,i) ∈ mem_locks (cmap_alter Γ g a m) ↔
@@ -988,7 +1039,7 @@ Lemma mem_locks_alter Γ Γm g a m w τ o i :
     (o,i) ∈ mem_locks m ∧ o = addr_index a ∧
       addr_object_offset Γ a + bit_size_of Γ τ ≤ i.
 Proof.
-  unfold lookupE, cmap_lookup; intros ? Hm ???.
+  unfold lookupE, cmap_lookup, lookupE, cmap_lookup_ref; intros ? Hm ???.
   case_option_guard; simplify_equality'.
   erewrite addr_object_offset_alt by eauto.
   destruct (cmap_car m !! addr_index a) as [[|w' β]|] eqn:?; simplify_equality'.
@@ -1055,7 +1106,8 @@ Lemma mem_Readable_locks Γ Γm m a w τ i :
   (addr_index a,i) ∈ mem_locks m →
   i < addr_object_offset Γ a ∨ addr_object_offset Γ a + bit_size_of Γ τ ≤ i.
 Proof.
-  unfold lookupE, cmap_lookup. rewrite elem_of_mem_locks.
+  unfold lookupE, cmap_lookup, lookupE, cmap_lookup_ref.
+  rewrite elem_of_mem_locks.
   intros ? Hm Hw ???; case_option_guard; simplify_equality'.
   destruct (decide (addr_object_offset Γ a ≤ i
     < addr_object_offset Γ a + bit_size_of Γ τ)) as [Hi|]; [exfalso|lia].
@@ -1107,17 +1159,27 @@ Lemma mem_locks_force Γ Γm a m v τ :
   ✓ Γ → ✓{Γ,Γm} m → (Γ,Γm) ⊢ a : Some τ →
   m !!{Γ} a = Some v → mem_locks (mem_force Γ a m) = mem_locks m.
 Proof.
-  unfold lookupE, mem_lookup, mem_force;
-    rewrite bind_Some; intros ??? (w&?&?); simplify_option_equality.
-  apply elem_of_equiv_L; intros [o i]; erewrite mem_locks_alter by eauto.
+  unfold lookupE, mem_lookup, mem_force, lookupE, cmap_lookup; intros.
+  case_option_guard; simplify_equality'.
+  destruct (m !!{Γ} _) as [w|] eqn:?; simplify_equality'.
+  destruct (cmap_lookup_ref_Some Γ Γm m (addr_index a)
+    (addr_ref Γ a) w) as (τ'&σ&?&?&?); eauto.
+  apply elem_of_equiv_L; intros [o i].
+  erewrite mem_locks_alter_ref
+    by eauto using addr_typed_index, addr_typed_ref_typed.
   destruct (decide (o = addr_index a)) as [->|]; [|tauto].
-  destruct (decide (addr_object_offset Γ a ≤ i
-    < addr_object_offset Γ a + bit_size_of Γ τ));
-    [|destruct (decide (i < addr_object_offset Γ a)); intuition omega].
-  rewrite pbits_Readable_locked by auto.
-  assert ((addr_index a,i) ∈ mem_locks m →
-    i < addr_object_offset Γ a ∨ addr_object_offset Γ a + bit_size_of Γ τ ≤ i)
-    by eauto using mem_Readable_locks; intuition congruence.
+  destruct (decide (ref_object_offset Γ (addr_ref Γ a) ≤ i
+    < ref_object_offset Γ (addr_ref Γ a) + bit_size_of Γ σ)).
+  { rewrite 2!or_r, or_l, elem_of_mem_locks by intuition lia.
+    unfold lookupE, cmap_lookup_ref in *; simplify_equality'.
+    destruct (cmap_car m !! _) as [[|w' malloc]|] eqn:?; simplify_equality'.
+    destruct (cmap_valid_Obj Γ Γm m (addr_index a) w' malloc)
+      as (?&?&_&?&_&_); simplify_type_equality'; eauto.
+    erewrite <-ctree_lookup_flatten by eauto.
+    rewrite <-list_lookup_fmap, pbits_locked_mask, list_lookup_fmap.
+    rewrite lookup_take, lookup_drop, le_plus_minus_r by lia.
+    intuition lia. }
+  destruct (decide (i < ref_object_offset Γ (addr_ref Γ a))); intuition omega.
 Qed.
 Lemma mem_locks_insert Γ Γm a m v τ :
   ✓ Γ → ✓{Γ,Γm} m → (Γ,Γm) ⊢ a : Some τ → mem_writable Γ a m → (Γ,Γm) ⊢ v : τ →
