memory_map_separation.v
@@ -11,11 +11,7 @@ Implicit Types τ σ : type Ti.
 Implicit Types w : mtree Ti.
 Implicit Types a : addr Ti.
 Implicit Types g : mtree Ti → mtree Ti.
-
-Arguments lookupE _ _ _ _ _ _ _ !_ /.
-Arguments cmap_lookup _ _ _ _ !_ /.
 Hint Extern 0 (Separation _) => apply (_ : Separation (pbit Ti)).
-Local Opaque nmap.Nempty.
 
 Lemma cmap_valid_subseteq Γ Γm m1 m2 : ✓ Γ → ✓{Γ,Γm} m2 → m1 ⊆ m2 → ✓{Γ,Γm} m1.
 Proof.
@@ -28,37 +24,70 @@ Proof.
     destruct Hm as [[??]?], (Hm2' o w' malloc') as (τ'&?&?&?&?);
       eauto 10 using ctree_typed_subseteq.
 Qed.
+Lemma cmap_lookup_ref_disjoint Γ Γm m1 m2 o r w1 w2 :
+  ✓ Γ → ✓{Γ,Γm} m1 → ✓{Γ,Γm} m2 → m1 ⊥ m2 →
+  m1 !!{Γ} (o,r) = Some w1 → m2 !!{Γ} (o,r) = Some w2 → w1 ⊥ w2.
+Proof.
+  destruct m1 as [m1], m2 as [m2]; intros ??? Hm ??; simplify_equality'.
+  specialize (Hm o).
+  destruct (m1 !! o) as [[|w1' β]|] eqn:Hw1,
+    (m2 !! o) as [[|w2' β']|] eqn:Hw2; simplify_equality'.
+  destruct (cmap_valid_Obj Γ Γm (CMap m1) o w1' β) as (τ&?&?&?&_),
+    (cmap_valid_Obj Γ Γm (CMap m2) o w2' β') as (?&?&?&?&_);
+    simplify_type_equality'; intuition eauto 3 using ctree_lookup_disjoint.
+Qed.
 Lemma cmap_lookup_disjoint Γ Γm m1 m2 a w1 w2 :
   ✓ Γ → ✓{Γ,Γm} m1 → ✓{Γ,Γm} m2 → m1 ⊥ m2 →
   m1 !!{Γ} a = Some w1 → m2 !!{Γ} a = Some w2 → w1 ⊥ w2.
 Proof.
-  destruct m1 as [m1], m2 as [m2]; simpl.
-  intros ? Hm1 Hm2 Hm ??. case_option_guard; simplify_equality'.
-  specialize (Hm (addr_index a)).
-  destruct (m1 !! addr_index a) as [[|w1' β]|] eqn:Hw1; simplify_equality'.
-  destruct (m2 !! addr_index a) as [[|w2' β']|] eqn:Hw2; simplify_equality'.
-  destruct (w1' !!{Γ} addr_ref Γ a) as [w1''|] eqn:?; simplify_equality'.
-  destruct (w2' !!{Γ} addr_ref Γ a) as [w2''|] eqn:?; simplify_equality'.
-  destruct (cmap_valid_Obj Γ Γm (CMap m1) (addr_index a) w1' β) as (τ&?&?&?&_),
-    (cmap_valid_Obj Γ Γm (CMap m2) (addr_index a) w2' β') as (?&?&?&?&_);
-    auto; simplify_type_equality'.
-  simplify_option_equality; naive_solver
-    eauto 3 using ctree_lookup_byte_disjoint, ctree_lookup_disjoint.
+  unfold lookupE, cmap_lookup; intros; case_option_guard; simplify_equality'.
+  destruct (m1 !!{_} _) as [w1'|] eqn:Hw1,
+    (m2 !!{_} _) as [w2'|] eqn:Hw2; simplify_option_equality;
+    eauto 3 using ctree_lookup_byte_disjoint, cmap_lookup_ref_disjoint.
+Qed.
+Lemma cmap_lookup_ref_subseteq Γ m1 m2 o r w1 :
+  ✓ Γ → m1 ⊆ m2 → m1 !!{Γ} (o,r) = Some w1 → ¬ctree_Forall sep_unmapped w1 →
+  ∃ w2, m2 !!{Γ} (o,r) = Some w2 ∧ w1 ⊆ w2.
+Proof.
+  destruct m1 as [m1], m2 as [m2]; simpl; intros ? Hm ??; specialize (Hm o).
+  destruct (m1 !! o) as [[|w1' β]|] eqn:?,
+    (m2 !! o) as [[|w2' β']|] eqn:?; simplify_equality'; try done.
+  destruct (ctree_lookup_subseteq Γ w1' w2' r w1)
+    as (w2''&?&?); simplify_option_equality; intuition eauto.
 Qed.
 Lemma cmap_lookup_subseteq Γ m1 m2 a w1 :
   ✓ Γ → m1 ⊆ m2 → m1 !!{Γ} a = Some w1 → ¬ctree_Forall sep_unmapped w1 →
   ∃ w2, m2 !!{Γ} a = Some w2 ∧ w1 ⊆ w2.
 Proof.
-  destruct m1 as [m1], m2 as [m2]; simpl.
-  intros ? Hm ??. case_option_guard; simplify_equality'.
-  specialize (Hm (addr_index a)).
-  destruct (m1 !! (addr_index a)) as [[|w1' β]|] eqn:?,
-    (m2 !! (addr_index a)) as [[|w2' β']|] eqn:?; simplify_equality'; try done.
-  destruct (w1' !!{Γ} addr_ref Γ a) as [w1''|] eqn:?; simplify_equality'.
-  destruct (ctree_lookup_subseteq Γ w1' w2' (addr_ref Γ a) w1'')
-    as (w2''&?&?); simplify_option_equality; intuition eauto using
-    ctree_lookup_byte_Forall, pbit_unmapped_indetify,ctree_lookup_byte_subseteq.
-  exfalso; eauto using @ctree_unshared_weaken.
+  unfold lookupE, cmap_lookup; intros; case_option_guard; simplify_equality'.
+  destruct (m1 !!{_} _) as [w1'|] eqn:Hw1; simplify_equality'.
+  assert (¬ctree_unmapped w1').
+  { simplify_option_equality; eauto using
+      ctree_lookup_byte_Forall, pbit_unmapped_indetify. }
+  destruct (cmap_lookup_ref_subseteq Γ m1 m2 (addr_index a)
+    (addr_ref Γ a) w1') as (w2'&->&?); simpl; auto.
+  simplify_option_equality by eauto using @ctree_unshared_weaken;
+    eauto using ctree_lookup_byte_subseteq.
+Qed.
+Lemma cmap_alter_ref_disjoint Γ Γm1 m1 m2 g o r w1 :
+  ✓ Γ → ✓{Γ,Γm1} m1 → m1 ⊥ m2 →
+  m1 !!{Γ} (o,r) = Some w1 → ¬ctree_unmapped (g w1) →
+  (∀ w2, w1 ⊥ w2 → g w1 ⊥ w2) → cmap_alter_ref Γ g o r m1 ⊥ m2.
+Proof.
+  assert (∀ w', ctree_empty w' → ctree_unmapped w').
+  { eauto using Forall_impl, @sep_unmapped_empty_alt. }
+  destruct m1 as [m1], m2 as [m2]; simpl; intros ? Hm1 Hm ??? o'.
+  specialize (Hm o'); destruct (decide (o' = o)); simplify_map_equality'; auto.
+  destruct (m1 !! o) as [[|w1' β]|] eqn:?; simplify_equality'; auto.
+  destruct (cmap_valid_Obj Γ Γm1 (CMap m1) o w1' β)
+    as (τ&?&_&?&_); auto; simplify_equality'.
+  destruct (m2 !! o) as [[|w2' β']|]; simplify_equality; auto.
+  { intuition eauto using ctree_alter_disjoint, ctree_alter_lookup_Forall. }
+  assert (∃ w2', w1' ⊥ w2') as (w2'&?).
+  { exists (ctree_new Γ ∅ τ); symmetry. eauto using ctree_new_disjoint. }
+  split.
+  { eapply ctree_disjoint_valid_l, ctree_alter_disjoint; intuition eauto. }
+  intuition eauto using ctree_alter_lookup_Forall.
 Qed.
 Lemma cmap_alter_disjoint Γ Γm1 m1 m2 g a w1 τ1 :
   ✓ Γ → ✓{Γ,Γm1} m1 → m1 ⊥ m2 →
@@ -68,58 +97,50 @@ Lemma cmap_alter_disjoint Γ Γm1 m1 m2 g a w1 τ1 :
 Proof.
   assert (∀ w', ctree_empty w' → ctree_unmapped w').
   { eauto using Forall_impl, @sep_unmapped_empty_alt. }
-  destruct m1 as [m1], m2 as [m2]; simpl. intros ? Hm1 Hm ????? o.
-  specialize (Hm o). case_option_guard; simplify_type_equality'.
-  destruct (decide (o = addr_index a)); simplify_map_equality'; [|apply Hm].
-  destruct (m1 !! addr_index a) as [[|w1' β]|] eqn:?; simplify_equality'.
-  destruct (w1' !!{Γ} addr_ref Γ a) as [w1''|] eqn:?; simplify_equality'.
-  destruct (cmap_valid_Obj Γ Γm1 (CMap m1) (addr_index a) w1' β)
+  unfold lookupE, cmap_lookup; intros; case_option_guard; simplify_equality'.
+  destruct (m1 !!{_} _) as [w1'|] eqn:Hw1; simplify_equality'.
+  destruct (cmap_lookup_ref_Some Γ Γm1 m1 (addr_index a) (addr_ref Γ a) w1')
+    as (τ&σ&?&?&?); auto.
+  eapply cmap_alter_ref_disjoint; eauto.
+  { simplify_option_equality; eauto.
+    assert (τ1 = ucharT%T) by eauto using addr_not_is_obj_type; subst.
+    intuition eauto 3 using ctree_alter_byte_unmapped. }
+  intros; simplify_option_equality; eauto using ctree_alter_byte_disjoint.
+Qed.
+Lemma cmap_alter_ref_union Γ Γm1 m1 m2 g o r w1 τ1 :
+  ✓ Γ → ✓{Γ,Γm1} m1 → m1 ⊥ m2 →
+  m1 !!{Γ} (o,r) = Some w1 → ¬ctree_unmapped (g w1) →
+  (∀ w2, w1 ⊥ w2 → g w1 ⊥ w2) → (∀ w2, w1 ⊥ w2 → g (w1 ∪ w2) = g w1 ∪ w2) →
+  cmap_alter_ref Γ g o r (m1 ∪ m2) = cmap_alter_ref Γ g o r m1 ∪ m2.
+Proof.
+  destruct m1 as [m1], m2 as [m2]; simpl; intros ? Hm1 Hm ????.
+  unfold union at 2, sep_union; f_equal'; apply map_eq; intros o'.
+  specialize (Hm o'); destruct (decide (o' = o)); simplify_map_equality';
+    rewrite !lookup_union_with, ?lookup_alter,
+    ?lookup_alter_ne, ?lookup_union_with by done; auto.
+  destruct (m1 !! o) as [[|w1' β]|] eqn:?; simplify_equality'; auto.
+  destruct (cmap_valid_Obj Γ Γm1 (CMap m1) o w1' β)
     as (τ&?&_&?&_); auto; simplify_equality'.
-  destruct (ctree_lookup_Some Γ Γm1 w1' τ (addr_ref Γ a) w1'')
-    as (τ'&_&?); auto.
-  destruct (m2 !! addr_index a) as [[|w2' ?]|] eqn:?; try done.
-  * destruct Hm as [(?&?&?)?]; case_decide; simplify_option_equality.
-    { split_ands; eauto using ctree_alter_disjoint, ctree_alter_lookup_Forall. }
-    assert (τ1 = ucharT%T) by eauto using addr_not_is_obj_type.
-    simplify_equality; split_ands; auto.
-    { eapply ctree_alter_disjoint; intuition eauto 3
-        using ctree_alter_byte_unmapped, ctree_alter_byte_disjoint. }
-    intuition eauto using ctree_alter_byte_unmapped, ctree_alter_lookup_Forall.
-  * assert (∃ w2', w1' ⊥ w2') as (w2'&?).
-    { exists (ctree_new Γ ∅ τ); symmetry. eauto using ctree_new_disjoint. }
-    destruct Hm. case_decide; simplify_option_equality.
-    { intuition eauto using ctree_alter_disjoint, ctree_alter_lookup_Forall,
-        @ctree_disjoint_valid_l, ctree_alter_disjoint. }
-    assert (τ1 = ucharT%T) by eauto using addr_not_is_obj_type.
-    simplify_equality. split.
-    { eapply ctree_disjoint_valid_l, ctree_alter_disjoint; intuition eauto 3
-        using ctree_alter_byte_disjoint, ctree_alter_byte_unmapped. }
-    intuition eauto using ctree_alter_byte_unmapped, ctree_alter_lookup_Forall.
+  destruct (m2 !! o) as [[|w2' β']|]; simplify_equality'; do 2 f_equal'.
+  intuition eauto using ctree_alter_union.
 Qed.
 Lemma cmap_alter_union Γ Γm1 m1 m2 g a w1 τ1 :
-  ✓ Γ → ✓{Γ,Γm1} m1 → m1 ⊥ m2 →
-  (Γ,Γm1) ⊢ a : Some τ1 → m1 !!{Γ} a = Some w1 → (Γ,Γm1) ⊢ g w1 : τ1 →
-  ¬ctree_unmapped (g w1) →
+  ✓ Γ → ✓{Γ,Γm1} m1 → m1 ⊥ m2 → (Γ,Γm1) ⊢ a : Some τ1 →
+  m1 !!{Γ} a = Some w1 → (Γ,Γm1) ⊢ g w1 : τ1 → ¬ctree_unmapped (g w1) →
   (∀ w2, w1 ⊥ w2 → g w1 ⊥ w2) → (∀ w2, w1 ⊥ w2 → g (w1 ∪ w2) = g w1 ∪ w2) →
   cmap_alter Γ g a (m1 ∪ m2) = cmap_alter Γ g a m1 ∪ m2.
 Proof.
-  destruct m1 as [m1], m2 as [m2]; unfold union, sep_union; simpl.
-  intros ? Hm1 Hm ??????; f_equal; apply map_eq; intros o.
-  case_option_guard; simplify_type_equality'.
-  destruct (decide (addr_index a = o)) as [<-|?]; rewrite !lookup_union_with,
-    ?lookup_alter, ?lookup_alter_ne, ?lookup_union_with by done; auto.
-  specialize (Hm (addr_index a)).
-  destruct (m1 !! addr_index a) as [[|w1' β]|] eqn:?,
-    (m2 !! addr_index a) as [[|w2' ?]|]; simplify_equality'; do 2 f_equal.
-  destruct (w1' !!{Γ} addr_ref Γ a) as [w1''|] eqn:?; simplify_equality'.
-  destruct (cmap_valid_Obj Γ Γm1 (CMap m1) (addr_index a) w1' β)
-    as (τ&?&_&?&_); auto; simplify_equality'.
-  destruct (ctree_lookup_Some Γ Γm1 w1' τ (addr_ref Γ a) w1'') as (τ'&_&?); auto.
-  destruct Hm as [(?&?&?)?]; case_decide; simplify_option_equality.
-  { eauto using ctree_alter_union. }
-  assert (τ1 = ucharT%T) by eauto using addr_not_is_obj_type.
-  simplify_equality. eapply ctree_alter_union; intuition eauto 3 using
-   ctree_alter_byte_disjoint, ctree_alter_byte_union, ctree_alter_byte_unmapped.
+  unfold lookupE, cmap_lookup, cmap_alter;
+    intros; case_option_guard; simplify_equality'.
+  destruct (m1 !!{_} _) as [w1'|] eqn:Hw1; simplify_equality'.
+  destruct (cmap_lookup_ref_Some Γ Γm1 m1 (addr_index a) (addr_ref Γ a) w1')
+    as (τ&σ&?&?&?); auto.
+  eapply cmap_alter_ref_union; eauto.
+  * simplify_option_equality; eauto.
+    assert (τ1 = ucharT%T) by eauto using addr_not_is_obj_type; subst.
+    intuition eauto 3 using ctree_alter_byte_unmapped.
+  * intros; simplify_option_equality; eauto using ctree_alter_byte_disjoint.
+  * intros; simplify_option_equality; eauto using ctree_alter_byte_union.
 Qed.
 Lemma cmap_singleton_disjoint Γ Γm a malloc w1 w2 τ :
   ✓ Γ → (Γ,Γm) ⊢ a : Some τ → addr_strict Γ a →
